src/library/constants.h
@@ -84,7 +84,6 @@ name const & get_has_add_name();
 name const & get_has_add_add_name();
 name const & get_has_andthen_andthen_name();
 name const & get_has_bind_and_then_name();
-name const & get_has_bind_bind_name();
 name const & get_has_bind_seq_name();
 name const & get_has_div_name();
 name const & get_has_div_div_name();
