tests/lean/run/check_constants.lean
@@ -82,7 +82,6 @@ run_cmd script_check_id `has_add
 run_cmd script_check_id `has_add.add
 run_cmd script_check_id `has_andthen.andthen
 run_cmd script_check_id `has_bind.and_then
-run_cmd script_check_id `has_bind.bind
 run_cmd script_check_id `has_bind.seq
 run_cmd script_check_id `has_div
 run_cmd script_check_id `has_div.div
