tests/lean/run/rebind_bind.lean
@@ -1,0 +1,12 @@
+class mono_monad (m : Type) (α : out_param Type) :=
+(pure : α → m)
+(bind : m → (α → m) → m)
+
+export mono_monad (bind pure)
+
+instance : mono_monad bool bool :=
+{ pure := id, bind := λ b f, if b then f b else b }
+
+#eval do b ← tt,
+         b' ← ff,
+         mono_monad.pure _ b
